Wip: zcb owner rights.

proofs/zero_coupon_bond.v
@@ -123,10 +123,135 @@ Qed.
 Print zcb_steps_O_to_I.
 
 
-(* The owner's rights:
-1. If  current time < now + period -> the owner can trigger payment later.
-2. If current time  = now + period and the owner triggers -> the owner gets paid.
-*)
+
+(* The owner's rights *)
+
+
+Definition executed
+           (ctr : FinContract)
+           (s s' : State)
+           (at_ : Time) :=
+  exists s s',
+    step s s' /\
+    In ctr (m_contracts s) /\
+    In (Executed (ctr_id ctr)) (m_events s') /\
+    at_ = m_global_time s.
+
+Definition joins
+           (O : Address)
+           (ctr : FinContract)
+           (s1 s2 : State)
+           (at_ : Time) :=
+  exists s s', steps s1 s /\ steps s' s2 /\ executed ctr s s' at_.
+Print Result.
+Print execute.
+Definition generates
+           (ctr new_ctr : FinContract) (s : State) (O : Address) :=
+  exists result,
+    execute (ctr_primitive ctr) (ctr_scale ctr) (ctr_issuer ctr) O
+            (m_balance s) (m_global_time s) (m_gateway s) (ctr_id ctr)
+            (ctr_desc_id ctr) (m_fresh_id s) (m_ledger s) = Some result /\
+    In new_ctr (res_contracts result).
+
+Definition joins_generated
+           (O : Address)
+           (ctr : FinContract)
+           (s1 s2 : State)
+           (t_first t_second : Time) :=
+  exists s s' new_ctr, steps s1 s /\ steps s' s2 /\ executed ctr s s' t_first /\
+               joins O new_ctr s' s2 t_second /\ generates ctr new_ctr s O.
+
+
+Lemma oups:
+  forall s1 s2 ctr_id dsc_id now period I O sc ctr,
+    consistent_state s1 ->
+    ctr = finctr ctr_id dsc_id (zcb_desc now period) I O O sc ->
+    joins_generated O ctr s1 s2 now (now + period) ->
+    exists tr,
+      In tr (m_ledger s2) /\
+      tr_from tr = I /\
+      tr_to tr = O /\
+      tr_amount tr = sc * 11.
+Proof.
+
+
+(* Definition is_generated *)
+(*            (child parent : FinContract) *)
+(*            (s1 s2 : State) *)
+(*            (proposed_owner : Address) *)
+(*            (at_ : Time) := *)
+(*   exists s s' bal' ctrs' next' ledger', *)
+(*     steps s1 s /\ *)
+(*     step s s' /\ *)
+(*     steps s' s2 /\ *)
+(*     In parent (m_contracts s) /\ *)
+(*     ~ In (Executed (ctr_id ctr)) (m_events s') /\  *)
+(*     execute (ctr_primitive parent) (ctr_scale parent) (ctr_issuer parent) proposed_owner *)
+(*             (m_balance s) (m_global_time s) (m_gateway s) (ctr_id parent)  *)
+(*             (ctr_desc_id parent) (m_fresh_id s) (m_ledger s) = *)
+(*     Some (result bal' ctrs' next' ledger') /\ *)
+(*     In child ctrs' /\ at_ = m_global_time s. *)
+
+    
+(*     p_owner <> 0 /\ *)
+
+
+Lemma oups:
+  forall s1 s2 ctr_id dsc_id now period I O sc ctr,
+    consistent_state s1 ->
+    O <> 0 ->
+    (exists new_ctr, is_generated_and_executed new_ctr ctr s1 s2 O now) ->
+    exists tr,
+      In tr (m_ledger s2) /\
+      tr_ctr_id tr = ctr_id /\
+      tr_from tr = I /\
+      tr_to tr = O /\
+      tr_amount tr = sc * 11.
+Proof.
+  intros.
+  destruct H3 as [new_ctr H3].
+  destruct H as (s & s' & S1 & S & S2 & IN & OW & E).
+  induction S; subst s'.
+  - simpl in E. destruct E as [E | E]; try inversion E.
+    find_contradiction IN.
+    eapply steps_preserves_consistent_state; eauto.
+  - ctr_case_analysis ctr ctr0.
+    unfold exec_ctr_in_state_with_owner in H9.
+    rewrite H1 in H9. simpl in H9.
+    case_analysis H9.
+    case_analysis H13.
+    + eexists. split.
+      eapply steps_does_not_remove_transactions.
+      exact S2. simpl. subst ledger'. simpl. left. eauto.
+      repeat split; eauto. simpl. resolve_owner H4.
+    + destruct H3 as (gs & gs' & bal' & ctrs'' & x' & L & G1 & GS & G2 & GIN & EXEC & GEN & L').
+      rewrite H1 in EXEC. simpl in EXEC.
+      case_analysis EXEC.
+      case_analysis H13.
+      ++ eexists. split.
+         eapply steps_does_not_remove_transactions.
+         exact G2. simpl. subst ledger'. simpl. right. left. eauto.
+      repeat split; eauto. simpl. resolve_owner H4.
+
+
+Admitted. 
+
+
+
+Lemma zcb_step_I_to_O :
+  forall s1 s2 ctr_id dsc_id now period I O sc ctr,
+    is_executed ctr s1 s2 O ->
+    consistent_state s1 ->
+    ctr = finctr ctr_id dsc_id (zcb_desc now period) I O O sc ->
+    
+    exists tr,
+      In tr (m_ledger s2) /\
+      tr_ctr_id tr = ctr_id /\
+      tr_from tr = I /\
+      tr_to tr = O /\
+      tr_amount tr = sc * 11.
+Proof.
+
 
 Lemma zcb_step_I_to_O :
   forall s1 s2 ctr_id dsc_id now period I O sc ctr,
@@ -136,8 +261,7 @@ Lemma zcb_step_I_to_O :
     In ctr (m_contracts s1) ->
     In (Executed ctr_id) (m_events s2) ->
     O <> 0 ->
-    (m_global_time s1) > now + period - Δ ->
-    (m_global_time s2) > now + period + Δ ->
+    (m_global_time s2) > now + period - Δ ->
     exists tr,
       In tr (m_ledger s2) /\
       tr_ctr_id tr = ctr_id /\
@@ -152,26 +276,46 @@ Proof.
   - ctr_case_analysis ctr ctr0.
     subst ctr s2. simpl in *.
     destruct H3 as [H3 | H3]; try contradiction. clear H3.
-    + unfold exec_ctr_in_state_with_owner in H12.
-      simpl in H12. inversion H12. clear H12.
+    + unfold exec_ctr_in_state_with_owner in H11.
+      simpl in H11. inversion H11. clear H11.
       case_analysis H3.
-      case_analysis H13.
+      case_analysis H12.
       * simpl. eexists. split.
         ** left. eauto.
-        ** repeat split; trivial. simpl. resolve_owner H7.
+        ** repeat split; trivial. simpl. resolve_owner H6.
       * apply ltb_sound_false in H3.
         apply ltb_sound_false in H1.
         contradict H3. omega.
-  - ctr_case_analysis ctr ctr0. subst ctr s2. simpl in H9.
-    unfold zcb_desc in H9. inversion H9.
-  - ctr_case_analysis ctr ctr0. subst ctr s2. simpl in H9.
-    unfold zcb_desc in H9. inversion H9.
+  - ctr_case_analysis ctr ctr0. subst ctr s2.
+    unfold zcb_desc in H8. inversion H8.
+  - ctr_case_analysis ctr ctr0. subst ctr s2.
+    unfold zcb_desc in H8. inversion H8.
   - ctr_case_analysis ctr ctr0. subst ctr s2.
     simpl in H3.
     destruct H3 as [H3 | H3]; try inversion H3.
     find_contradiction H2.
   - subst. simpl in *. find_contradiction H2.
 Qed.
+
+
+Lemma zcb_steps_I_to_O :
+  forall s1 s2 ctr_id dsc_id now period I O sc ctr,
+    steps s1 s2 ->
+    consistent_state s1 ->
+    ctr = finctr ctr_id dsc_id (zcb_desc now period) I O O sc ->
+    In ctr (m_contracts s1) ->
+    In (Executed ctr_id) (m_events s2) ->
+    O <> 0 ->
+    (m_global_time s2) > now + period - Δ ->
+    exists s s', steps s1 s /\ step s s' /\ steps s' s2 /\ In 
+    exists tr,
+      In tr (m_ledger s2) /\
+      tr_ctr_id tr = ctr_id /\
+      tr_from tr = I /\
+      tr_to tr = O /\
+      tr_amount tr = sc * 11.
+Proof.
+
 
 Lemma zcb_step_I_to_O' :
   forall s1 s2 ctr_id dsc_id now period I O sc ctr,
@@ -181,7 +325,7 @@ Lemma zcb_step_I_to_O' :
     In ctr (m_contracts s1) ->
     In (Executed ctr_id) (m_events s2) ->
     O <> 0 ->
-    (m_global_time s2) < now + period - Δ ->
+    (m_global_time s1) <= now + period - Δ ->
     exists ctr,
       In ctr (m_contracts s2) /\
       ctr_primitive ctr = (At (now + period) (Scale 11 (One USD))) /\
@@ -197,18 +341,18 @@ Proof.
     subst ctr s2. simpl in *.
     destruct H3 as [H3 | H3]; try contradiction.
     + unfold exec_ctr_in_state_with_owner in *.
-      simpl in H12. inversion H12.
-      case_analysis H12.
-      case_analysis H15.
+      simpl in H11. inversion H11.
+      case_analysis H11.
+      case_analysis H14.
       * apply ltb_sound_true in H12.
         apply ltb_sound_false in H1.
         omega.
       * eexists. split; simpl.
         ** rewrite in_app_iff. right. simpl. left. eauto.
         ** repeat split; trivial. resolve_owner H6.
-  - ctr_case_analysis ctr ctr0. subst ctr s2. simpl in H8.
+  - ctr_case_analysis ctr ctr0. subst ctr s2.
     unfold zcb_desc in H8. inversion H8.
-  - ctr_case_analysis ctr ctr0. subst ctr s2. simpl in H8.
+  - ctr_case_analysis ctr ctr0. subst ctr s2.
     unfold zcb_desc in H8. inversion H8.
   - ctr_case_analysis ctr ctr0. subst ctr s2.
     simpl in H3.
@@ -218,22 +362,132 @@ Proof.
 Qed.
 
 
-Lemma zcb_steps_I_to_O':
-  forall s1 s2 ctr_id dsc_id now period I O sc ctr,
-    steps s1 s2 ->
+
+
+
+
+
+
+(*
+
+
+
+
+WHOAAAA
+
+ *)
+
+
+
+Lemma zcb_step_I_to_O'' :
+  forall s1 s2 ctr_id dsc_id period I O sc ctr,
+    step s1 s2 ->
     consistent_state s1 ->
-    ctr = finctr ctr_id dsc_id (zcb_desc now period) I O O sc ->
+    ctr = finctr ctr_id dsc_id (zcb_desc (m_global_time s1) period) I O O sc ->
     In ctr (m_contracts s1) ->
     In (Executed ctr_id) (m_events s2) ->
     O <> 0 ->
-    (m_global_time s1) > now + period + Δ ->
-    (m_global_time s2) < now + period - Δ ->
-    exists ctr,
-      In ctr (m_contracts s2) /\
-      ctr_primitive ctr = (At (now + period) (Scale 11 (One USD))) /\
-      ctr_issuer ctr = I /\
-      ctr_proposed_owner ctr = O /\
-      ctr_scale ctr = sc.
+    (m_global_time s2) > (m_global_time s1) + period - Δ ->
+    exists tr,
+      In tr (m_ledger s2) /\
+      tr_ctr_id tr = ctr_id /\
+      tr_from tr = I /\
+      tr_to tr = O /\
+      tr_amount tr = sc * 11.
+Proof.
+  intros.
+  induction H.
+  - subst s2. find_contradiction H2.
+    destruct H3 as [H3 | H3]; try inversion H3; try contradiction.
+  - ctr_case_analysis ctr ctr0.
+    subst ctr s2. simpl in *.
+    destruct H3 as [H3 | H3]; try contradiction. clear H3.
+    unfold exec_ctr_in_state_with_owner in H11.
+    simpl in H11. inversion H11. clear H11.
+    case_analysis H3.
+    case_analysis H11.
+    * eexists. split.
+      ** simpl. left. eauto.
+      ** repeat split; trivial. resolve_owner H6.
+    *  apply ltb_sound_false in H1.
+       apply ltb_sound_false in H3.
+       contradict H3. omega.
+  - ctr_case_analysis ctr ctr0. subst ctr s2.
+    unfold zcb_desc in H8. inversion H8.
+  - ctr_case_analysis ctr ctr0. subst ctr s2.
+    unfold zcb_desc in H8. inversion H8.
+  - ctr_case_analysis ctr ctr0. subst ctr s2.
+    simpl in H3.
+    destruct H3 as [H3 | H3]; try inversion H3.
+    find_contradiction H2.
+  - subst. simpl in *. find_contradiction H2.
+Qed.
+
+
+Lemma gt_implies_ge_Sn :
+  forall n m,
+    n > m -> n >= S m.
+Admitted.
+
+Lemma ge_implies_eq_or_gt:
+  forall n m,
+    n >= m -> n = m \/ n > m.
+Admitted.
+
+
+
+Lemma helper1 :
+  forall s1 s2 ctr period O,
+    steps s1 s2 ->
+    In ctr (m_contracts s1) ->
+    consistent_state s1 ->
+    In (Executed (ctr_id ctr)) (m_events s2) ->
+    ctr_primitive ctr = zcb_desc (m_global_time s1) period ->
+    O <> 0 ->
+    m_global_time s2 > m_global_time s1 + period -  Δ.
+Proof.
+  intros.
+  induction H.
+  - subst s2. find_contradiction H2.
+  - assert (H' := H). assert (H'' := H).
+    apply steps_preserves_consistent_state in H'; auto.
+    apply steps_effect_over_contract with (ctr := ctr) in H; trivial.
+    destruct H as [H|[H|H]]; trivial.
+    + induction H5; subst s2; simpl.
+      ++ simpl in H2. destruct H2 as [H2 | H2]; try inversion H2.
+         find_contradiction H0.
+      ++ ctr_case_analysis ctr ctr0.
+         simpl in H2. destruct H2 as [H2 | H2]; try contradiction. clear H2.
+         unfold exec_ctr_in_state_with_owner in H11. rewrite H3 in H11.
+         simpl in H11.
+         case_analysis H11.
+         case_analysis H14.
+         ** apply ltb_sound_true in H11. auto.
+         ** apply ltb_sound_false in H11.
+            apply ltb_sound_false in H2.
+         
+
+    + eapply IHsteps in H. admit.
+    + admit.
+Admitted.
+
+
+Lemma zcb_steps_I_to_O'' :
+  forall s1 s2 ctr_id dsc_id period I O sc ctr,
+    steps s1 s2 ->
+    consistent_state s1 ->
+    ctr = finctr ctr_id dsc_id (zcb_desc (m_global_time s1) period) I O O sc ->
+    In ctr (m_contracts s1) ->
+    In (Executed ctr_id) (m_events s2) ->
+    O <> 0 ->
+    period - Δ > 0 ->
+    (m_global_time s2) > (m_global_time s1) + period - Δ ->
+    exists tr,
+      In tr (m_ledger s2) /\
+      tr_ctr_id tr = ctr_id /\
+      tr_from tr = I /\
+      tr_to tr = O /\
+      tr_amount tr = sc * 11.
 Proof.
   intros.
   induction H.
@@ -242,394 +496,59 @@ Proof.
     apply steps_preserves_consistent_state in H'; auto.
     apply steps_effect_over_contract with (ctr := ctr) in H; trivial.
     destruct H as [H|[H|H]]; trivial.
-    + eapply zcb_step_I_to_O'; eauto.
-    + assert (S := H6).
-      apply time_inc in H6.
-      assert (m_global_time s <= now + period - Δ); try omega.
-      subst ctr. simpl in *.
-      apply IHsteps in H; auto.
-      destruct H as [ctr [H [A HT]]].
-      exists ctr.
+    + eapply zcb_step_I_to_O; eauto.
+    + rewrite H1 in H. simpl in H.
+      eapply helper1 with (period := period) in H''; eauto.
+      ++ eapply IHsteps in H''; eauto.
+         destruct H'' as [tr [H'' H''']].
+         eexists. split; eauto.
+         eapply step_does_not_remove_transactions; eauto.
+      ++ subst ctr. trivial.
+      ++ subst ctr. trivial.
+    + assert (C := H7). rewrite H1 in H. simpl in H.
+      eapply step_preserves_consistent_state in C; eauto.
+      eapply step_does_not_remove_events in H7.
+      unfold consistent_state in C.
+      destruct C as [_ [_ [_ [_ C]]]].
+      unfold not in C.
+      exfalso. eapply C; eauto.
+      trivial.
+Admitted.
+
+
+
+      assert (HT := H7).
+      assert (N : m_global_time s > m_global_time s1 + period + Δ).
+      {
+        induction H''; intros.
+        - subst s0. find_contradiction H.
+        - induction H8; subst s0.
+          + simpl in *. destruct H as [H | H]; try inversion H.
+            apply IHH'' in H; auto.
+
+
+        }
+      eapply timebound_steps in H; eauto.
+
+      apply gt_implies_ge_Sn in H6.
+      eapply time_passes_one_step_at_a_time in H6; eauto.
+      apply ge_implies_eq_or_gt in H6.
+      destruct H6 as [H6 | H6].
+      ++ rewrite H6 in *.
+
+      eapply zcb_step_I_to_O''; eauto.
+    + subst ctr. simpl in *.
+      apply IHsteps in H.
+      destruct H as [tr [H HT]].
+      exists tr.
       split; trivial.
-      ++ induction S; subst s2; simpl; auto.
-         ** ctr_case_analysis ctr ctr0.
-            destruct ctr. simpl in *.
-            rewrite A in H13.
-            clear H14 H12 H10 H9 IHsteps H12 H3 H4 H1 H8 H2 H A HT.
-            unfold exec_ctr_in_state_with_owner in H13. simpl in *.
-            case_if H13.
-            case_if H17.
-            *** apply ltb_sound_true in H1.
-                apply ltb_sound_false in H.
-                omega.
-            *** apply ltb_sound_false in H1.
-                apply ltb_sound_false in H. 
-                contradict H13. auto.
-
-            destruct (ctr_primitive ctr); try inversion A.
-            subst. simpl in H5, H6.
-
-
-        struct (ctr_primitive ctr); inversion A.
-         subst. 
-         
-
-      admit.
+      eapply step_does_not_remove_transactions; eauto.
     + eapply step_preserves_consistent_state in H'; eauto.
-      eapply step_does_not_remove_events in H6; eauto.
+      eapply step_does_not_remove_events in H5; eauto.
       destruct H' as [_ [_ [_ [_ T]]]].
       unfold not in T.
       exfalso.
       eapply T. subst ctr.
       split; eauto.
-Admitted.
-
-Lemma timebound_postpone:
-  forall s s' c p t0 t1,
-    step s s' ->
-    consistent_state s ->
-    In c (m_contracts s) ->
-    m_global_time s <= t0 ->
-    m_global_time s' <= t0 ->
-    ctr_primitive c = (Timebound t0 t1 p) ->
-    exists c', In c' (m_contracts s') /\ ctr_primitive c' = p.
-Proof.
-  intros.
-  induction H; subst s'; simpl.
-  - right. trivial.
-  - ctr_case_analysis c ctr.
-    apply in_app_iff.
-    unfold exec_ctr_in_state_with_owner in H8.
-    induction (ctr_primitive c); simpl in *; try inversion H3.
-    subst. 
-    clear H6 H.
-    subst.
-    clear H10 H3.
-    
-    + apply ltb_sound_true in H9.
-      apply ltb_sound_false in H12.
-      try omega.
-    + simpl. subst.
-      clear H2 H5 H0.
-
-
-
-
-(* Failed attempt: cannot prove that the owner always gets paid! *)
-Lemma zcb_execute_I_to_O :
-  forall sc now period I O bal time gtw ctr_id dsc_id next_id ledger result,
-    execute (zcb_desc now period)  sc I O bal time gtw ctr_id dsc_id next_id ledger =
-    Some result ->
-    exists tr,
-      In tr (res_ledger result) /\
-      tr_ctr_id tr = ctr_id /\
-      tr_from tr = I /\
-      tr_to tr = O /\
-      tr_amount tr = sc * 11 /\
-      tr_timestamp tr = time.
-Proof.
-  unfold zcb_desc. intros.
-  simpl in H.
-  case_analysis H.
-  case_analysis H2; simpl in *.
-  - eexists.
-    split.
-    + left. trivial.
-    + repeat split; trivial.
-  - admit. (* This case cannot be proved. Timebounds generates a new contract
-              whose execution can be triggered later.  *)
-Admitted.
-
-
-(* Contract execution either produces a transaction or a new contract. *) 
-Lemma zcb_execute_I_to_O_new_ctr :
-  forall sc now period I O bal time gtw ctr_id dsc_id next_id ledger result,
-    execute (zcb_desc now period)  sc I O bal time gtw ctr_id dsc_id next_id ledger =
-    Some result ->
-    (exists tr,
-      In tr (res_ledger result) /\
-      tr_ctr_id tr = ctr_id /\
-      tr_from tr = I /\
-      tr_to tr = O /\
-      tr_amount tr = sc * 11 /\
-      tr_timestamp tr = time) \/
-    exists ctr,
-      In ctr (res_contracts result) /\
-      ctr_primitive ctr = (At (now + period) (Scale 11 (One USD))) /\
-      ctr_issuer ctr = I /\
-      ctr_proposed_owner ctr = O /\
-      ctr_scale ctr = sc.
-Proof.
-  unfold zcb_desc. intros.
-  simpl in H.
-  case_analysis H.
-  case_analysis H2; simpl in *.
-  - left. eexists.
-    split.
-    + left. trivial.
-    + repeat split; trivial.
-  - right.
-    eexists. split.
-    + left. trivial.
-    + simpl. unfold At. repeat split; trivial.
 Qed.
 
-
-Lemma zcb_step_I_to_O :
-  forall s1 s2 ctr_id dsc_id now period I O sc ctr,
-    step s1 s2 ->
-    consistent_state s1 ->
-    ctr = finctr ctr_id dsc_id (zcb_desc now period) I O O sc ->
-    In ctr (m_contracts s1) ->
-    In (Executed ctr_id) (m_events s2) ->
-    O <> 0 ->
-    (exists tr,
-      In tr (m_ledger s2) /\
-      tr_ctr_id tr = ctr_id /\
-      tr_from tr = I /\
-      tr_to tr = O /\
-      tr_amount tr = sc * 11) \/
-    exists ctr,
-      In ctr (m_contracts s2) /\
-      ctr_primitive ctr = (At (now + period) (Scale 11 (One USD))) /\
-      ctr_issuer ctr = I /\
-      ctr_proposed_owner ctr = O /\
-      ctr_scale ctr = sc.
-Proof.
-  intros.
-  induction H; subst s2.
-  - simpl in *. destruct H3 as [H3 | H3]; try inversion H3.
-    find_contradiction H2.
-  - case_eq (ctr_eq_dec ctr ctr0); intros; try contradiction.
-    subst ctr0. simpl in *. destruct H3 as [H3 | H3].
-    + unfold exec_ctr_in_state_with_owner in H10.
-      rewrite H1 in H10. simpl in H10.
-      case_analysis H10.
-      case_analysis H14.
-      * left. eexists. split. simpl. left. trivial.
-        simpl. repeat split; trivial.
-        unfold can_join in H5.
-        destruct H5 as [H5 | H5]; subst; simpl in *; trivial.
-        subst O. contradiction.
-      * right. eexists. split. rewrite in_app_iff.
-        right. simpl. left. trivial.
-        simpl. repeat split; trivial.
-        unfold can_join in H5.
-        destruct H5 as [H5 | H5]; subst; simpl in *; trivial.
-        subst O. contradiction.
-    + subst ctr. simpl in *. contradiction.
-  - case_eq (ctr_eq_dec ctr ctr0); intros; try contradiction.
-    subst ctr0 ctr. unfold zcb_desc in *. simpl in H7. inversion H7.
-  - case_eq (ctr_eq_dec ctr ctr0); intros; try contradiction.
-    subst ctr0 ctr. unfold zcb_desc in *. simpl in H7. inversion H7.
-  - case_eq (ctr_eq_dec ctr ctr0); intros; try contradiction.
-    subst ctr0. simpl in *. destruct H3 as [H3 | H3]; try inversion H3.
-    apply consistent_impl_exec in H2; auto.
-    subst ctr. simpl in *. contradiction.
-  - subst. simpl in *.    
-    apply consistent_impl_exec in H2; auto.
-    simpl in *. contradiction.
-Qed.
-
-
-Lemma zcb_steps_I_to_O_new_ctr :
-  forall s1 s2 ctr_id dsc_id now period I O sc ctr,
-    steps s1 s2 ->
-    now + period + Δ <=? m_global_time s2 = false ->
-    consistent_state s1 ->
-    ctr = finctr ctr_id dsc_id (zcb_desc now period) I O O sc ->
-    In ctr (m_contracts s1) ->
-    In (Executed ctr_id) (m_events s2) ->
-    O <> 0 ->
-    (exists tr,
-      In tr (m_ledger s2) /\
-      tr_from tr = I /\
-      tr_to tr = O /\
-      tr_amount tr = sc * 11) \/
-    exists ctr,
-      In ctr (m_contracts s2) /\
-      ctr_primitive ctr = (At (now + period) (Scale 11 (One USD))) /\
-      ctr_issuer ctr = I /\
-      ctr_proposed_owner ctr = O /\
-      ctr_scale ctr = sc.
-Proof.
-  intros s1 s2 ctr_id0 dsc_id0 now period I O sc ctr H CH. intros.
-  assert (C : ~ In (Executed (ctr_id ctr)) (m_events s1)).
-  apply consistent_impl_exec; auto.
-  rewrite H1 in C. simpl in C.
-  induction H.
-  - subst. contradiction.
-  - assert (H' := H). assert (H'' := H).
-    apply steps_preserves_consistent_state in H'; auto.
-    apply steps_effect_over_contract with (ctr := ctr) in H; trivial.
-    destruct H as [H|[H|H]]; trivial.
-    + eapply zcb_step_I_to_O in H5; eauto.
-      destruct H5 as [(tr & A1 & A2 & A3 & A4 & A5) | H5]; auto.
-      left. exists tr. repeat split; trivial.
-    + rewrite H1 in H. simpl in H.
-      apply IHsteps in H.
-      destruct H as [H | H].
-      ++ left. destruct H as [tr [A1 [A2 A3]]].
-         exists tr. split; auto.
-         eapply steps_does_not_remove_transactions; eauto.
-         eapply tran; eauto. apply refl. trivial.
-      ++ clear IHsteps C H'' H1 H2 H3 H0.
-         destruct H as [ct [H HT]].
-         assert (CP := H5).
-         apply step_effect_over_contract with (ctr := ct) in H5; trivial.
-         destruct H5 as [H5 | [H5 | H5]].
-         ** right. exists ct. split; trivial.
-         ** induction CP.
-            *** subst s2. right. exists ct. split; trivial.
-                simpl. right. trivial.
-            *** case_eq (ctr_eq_dec ctr0 ct); intros; try contradiction.
-                subst ctr0.
-                unfold exec_ctr_in_state_with_owner in H8.
-                destruct HT as [HT [B1 [B2 B3]]].
-                rewrite HT in H8.
-                simpl in H8.
-                case_if H8.
-                case_if H12.
-                **** left. subst s2 ledger'. simpl.
-                     eexists. split. left. eauto. simpl.
-                     repeat split; trivial.
-                     unfold can_join in H1.
-                     destruct H1 as [H1 | H1].
-                     subst. trivial.
-                     subst. contradiction.
-                     rewrite B3. trivial.
-                **** right. subst s2 ctrs'. eexists.
-                     split; simpl.
-                     rewrite in_app_iff. right. simpl. left. eauto.
-                     simpl. unfold At. repeat split; auto.
-                     unfold can_join in H1.
-                     destruct H1 as [H1 | H1].
-                     subst. trivial.
-                     subst. contradiction.
-            *** case_eq (ctr_eq_dec ctr0 ct); intros; try contradiction.
-                subst ctr0. destruct HT as [HT [B1 [B2 B3]]].
-                rewrite HT in H3. inversion H3.
-            *** case_eq (ctr_eq_dec ctr0 ct); intros; try contradiction.
-                subst ctr0. destruct HT as [HT [B1 [B2 B3]]].
-                rewrite HT in H3. inversion H3.
-            *** case_eq (ctr_eq_dec ctr0 ct); intros; try contradiction.
-                subst ctr0. destruct HT as [HT [B1 [B2 B3]]].
-                subst s2. simpl in H5.
-                destruct H5 as [H5 | H5]; try inversion H5.
-                contradict H5.
-                apply consistent_impl_exec; auto.
-            *** subst s2. simpl in *. right.
-                exists ct. split; trivial.
-         ** induction CP.
-            *** subst s2. simpl in H5.
-                destruct H5 as [H5 | H5]; try inversion H5.
-                destruct H' as [_ [_ [_ [H' _]]]].
-                apply H' in H.
-                destruct H as [_ H].
-                contradiction.
-            *** case_eq (ctr_eq_dec ctr0 ct); intros; try contradiction.
-                subst ctr0. destruct HT as [HT [B1 [B2 B3]]].
-                subst s2. simpl in *.
-                destruct H5 as [H5 | H5]; try inversion H5.
-                destruct H' as [_ [_ [_ [H' _]]]].
-                apply H' in H.
-                destruct H as [_ H].
-                contradiction.
-            *** case_eq (ctr_eq_dec ctr0 ct); intros; try contradiction.
-                subst ctr0. destruct HT as [HT [B1 [B2 B3]]].
-                rewrite HT in H3. inversion H3.
-            *** case_eq (ctr_eq_dec ctr0 ct); intros; try contradiction.
-                subst ctr0. destruct HT as [HT [B1 [B2 B3]]].
-                rewrite HT in H3. inversion H3.
-            *** case_eq (ctr_eq_dec ctr0 ct); intros; try contradiction.
-                subst ctr0. destruct HT as [HT [B1 [B2 B3]]].
-                subst s2. simpl in *.
-                destruct H5 as [H5 | H5].
-                **** unfold exec_ctr_in_state_with_owner in H6.
-                     rewrite HT in H6.
-                     simpl in H6.
-                     case_if H6.
-                     unfold Nat.ltb in H7.
-                     apply leb_sound_true in H7.
-                     apply leb_sound_false in CH.
-                     exfalso.
-                     apply CH.
-                     omega.
-                     case_if H10.
-                **** destruct H' as [_ [_ [_ [H' _]]]].
-                     apply H' in H.
-                     destruct H as [_ H].
-                     contradiction.
-            *** subst s2. simpl in *. right.
-                exists ct. split; trivial.
-      ++ apply leb_sound_false in CH.
-         apply propleb_sound_false.
-         intros not.
-         apply CH.
-         apply time_inc in H5.
-         omega.
-    + eapply step_does_not_remove_events in H; eauto.
-      eapply step_preserves_consistent_state in H'; eauto.
-      subst ctr. simpl in H.
-      destruct H' as [_ [_ [_ [_ H']]]].
-      exfalso.
-      eapply H'; eauto.
-Qed.
-
-
-
-(* Lemma zcb_step_I_to_O' : *)
-(*   forall s1 s2 ctr_id dsc_id now period I O sc ctr, *)
-(*     step s1 s2 -> *)
-(*     consistent_state s1 -> *)
-(*     ctr = finctr ctr_id dsc_id (zcb_desc now period) I O O sc -> *)
-(*     In ctr (m_contracts s1) -> *)
-(*     In (Executed ctr_id) (m_events s2) -> *)
-(*     O <> 0 -> *)
-(*     (m_global_time s2) > now + period -> *)
-(*     (exists tr, *)
-(*       In tr (m_ledger s2) /\ *)
-(*       tr_ctr_id tr = ctr_id /\ *)
-(*       tr_from tr = I /\ *)
-(*       tr_to tr = O /\ *)
-(*       tr_amount tr = sc * 11). *)
-(* Proof. *)
-(* Admitted. *)
-
-(* Lemma zcb_steps_I_to_O' : *)
-(*   forall s1 s2 ctr_id dsc_id now period I O sc ctr, *)
-(*     steps s1 s2 -> *)
-(*     consistent_state s1 -> *)
-(*     ctr = finctr ctr_id dsc_id (zcb_desc now period) I O O sc -> *)
-(*     In ctr (m_contracts s1) -> *)
-(*     In (Executed ctr_id) (m_events s2) -> *)
-(*     O <> 0 -> *)
-(*     (m_global_time s2) > now + period -> *)
-(*     (m_global_time s1) = now -> *)
-(*     (exists tr, *)
-(*       In tr (m_ledger s2) /\ *)
-(*       tr_ctr_id tr = ctr_id /\ *)
-(*       tr_from tr = I /\ *)
-(*       tr_to tr = O /\ *)
-(*       tr_amount tr = sc * 11). *)
-(* Proof. *)
-(*   intros. *)
-(*   induction H. *)
-(*   - subst s2. omega. *)
-(*   - assert (Ss := H). assert (S := H7). *)
-(*     eapply steps_effect_over_contract in H; eauto. *)
-(*     eapply steps_preserves_consistent_state in Ss; eauto. *)
-(*     destruct H as [H | [H | H]]. *)
-(*     + eapply zcb_step_I_to_O' in S; eauto. *)
-(*     + rewrite H1 in H. simpl in H. *)
-(*       eapply IHsteps in H. *)
-(*       * destruct H as [tr [H H']]. *)
-(*         exists tr. split; trivial. *)
-(*         eapply step_does_not_remove_transactions; eauto. *)
-(*       * induction H7; subst s2. *)
-(*         ** find_contradiction H2. *)
-(*         ** ctr_case_analysis ctr ctr0. simpl in H5. trivial. *)
-(*         ** ctr_case_analysis ctr ctr0. simpl in H5. trivial. *)
-(*         ** ctr_case_analysis ctr ctr0. simpl in H5. trivial. *)
-(*         ** ctr_case_analysis ctr ctr0. simpl in H5. trivial. *)
-(*         ** simpl in *. f *)
